LeanSAT/Reflect/BVExpr/BitBlast/Impl/GetLsb.lean
@@ -1,0 +1,38 @@
+import LeanSAT.Reflect.BVExpr.BitBlast.Impl.Expr
+
+namespace BVPred
+
+structure GetLsbTarget where
+  {w : Nat}
+  expr : BVExpr w
+  idx : Nat
+
+def blastGetLsb (aig : AIG BVBit) (target : GetLsbTarget) : AIG.Entrypoint BVBit :=
+  if h:target.idx < target.w then
+    -- Note: This blasts the entire rexpression up to `w` despite only needing it up to `idx`.
+    -- However the vast majority of operations are interested in all bits so the API is currently
+    -- not designed to support this use case.
+    let res := target.expr.bitblast aig
+    let aig := res.aig
+    let stream := res.stream
+    ⟨aig, stream.getRef target.idx h⟩
+  else
+    AIG.mkConstCached aig false
+
+instance : AIG.LawfulOperator BVBit (fun _ => GetLsbTarget) blastGetLsb where
+  le_size := by
+    intros
+    unfold blastGetLsb
+    dsimp
+    split
+    . apply AIG.LawfulStreamOperator.le_size (f := BVExpr.bitblast)
+    . apply AIG.LawfulOperator.le_size (f := AIG.mkConstCached)
+  decl_eq := by
+    intros
+    unfold blastGetLsb
+    dsimp
+    split
+    . rw [AIG.LawfulStreamOperator.decl_eq (f := BVExpr.bitblast)]
+    . rw [AIG.LawfulOperator.decl_eq (f := AIG.mkConstCached)]
+
+end BVPred
