LeanSAT/Reflect/BVExpr/BitBlast/Lemmas/GetLsb.lean
@@ -1,0 +1,24 @@
+import LeanSAT.Reflect.BVExpr.BitBlast.Lemmas.Basic
+import LeanSAT.Reflect.BVExpr.BitBlast.Lemmas.Expr
+import LeanSAT.Reflect.BVExpr.BitBlast.Impl.GetLsb
+
+open AIG
+
+namespace BVPred
+
+@[simp]
+theorem blastGetLsb_denote_eq_eval_getLsb (aig : AIG BVBit) (target : GetLsbTarget) (assign : BVExpr.Assignment)
+    : ⟦blastGetLsb aig target, assign.toAIGAssignment⟧
+        =
+      (target.expr.eval assign).getLsb target.idx := by
+  rcases target with ⟨expr, idx⟩
+  unfold blastGetLsb
+  dsimp
+  split
+  . simp
+  . next h =>
+    simp only [mkConstCached_eval_eq_mkConst_eval, denote_mkConst, Bool.false_eq]
+    apply BitVec.getLsb_ge
+    omega
+
+end BVPred
